src/real/hol4-real-sat.thy
@@ -16,6 +16,7 @@ show: "Number.Real"
 show: "Relation"
 main {
   import: unsat
+  import: proofs
 }
 unsat {
   import: proofs
@@ -26,4 +27,8 @@ proofs {
   interpretation: "../opentheory/hol4.int"
   interpret: const "HOL4.prove_real_assums.real_0" as "HOL4.realax.real_0"
   interpret: const "HOL4.prove_real_assums.real_1" as "HOL4.realax.real_1"
+  interpret: const "HOL4.prove_real_assums.inv" as "Number.Real.inv"
+  interpret: const "HOL4.prove_real_assums.inv0" as "HOL4.realax.inv"
+  interpret: const "HOL4.prove_real_assums./" as "Number.Real./"
+  interpret: const "HOL4.prove_real_assums.real_div" as "HOL4.real./"
 }
